aneris/aneris_lang/adequacy_trace.v
@@ -1,0 +1,61 @@
+From aneris.aneris_lang Require Import aneris_lang proofmode adequacy_no_model.
+
+Definition heap_invariance `{anerisPreG Σ unit_model} (N : namespace) (I : list val → Prop) ip e σ :
+  I (state_trace σ) →
+  (∀ `(anerisG Σ), ⊢ trace_inv N I -∗ trace_is (state_trace σ) -∗ WP e @[ip] ⊤ {{ _, True }}) →
+  ∀ σ' t,
+    step ([(mkExpr ip e)], σ) (t, σ') →
+    I (state_trace σ').
+Proof.
+  (* intros HI Hwp σ' t.
+  eapply (wp_invariance Σ _ s _ _ _ _ (I (trace σ'))). iIntros (Hinv κs) "".
+  iMod (gen_heap_init σ.(heap)) as (?) "Hh".
+  iMod (proph_map_init κs σ.(used_proph_id)) as (?) "Hp".
+  iMod (trace_auth_init σ.(trace)) as (?) "(Hta & Ht & Hth)".
+  iDestruct (inv_alloc N _ (∃ t, trace_half_frag t ∗ ⌜I t⌝) with "[Hth]") as ">#HI".
+  { iNext. eauto. }
+  iModIntro. iExists
+    (λ σ κs _, (gen_heap_ctx σ.(heap) ∗ trace_auth σ.(trace) ∗ proph_map_ctx κs σ.(used_proph_id))%I),
+    (λ _, True%I).
+  iFrame. iSplitL.
+  { iDestruct (Hwp (HeapG _ _ _ _ _)) as "Hwp". iApply ("Hwp" with "HI Ht"). }
+  iIntros "(_ & Hta & _)". iExists _.
+  iInv "HI" as ">Ht'" "_". iDestruct "Ht'" as (t') "(Ht' & %)".
+  iDestruct (trace_auth_half_frag_agree with "Hta Ht'") as %->. iModIntro. eauto.
+Qed. *)
+Admitted.
+
+Lemma module_invariance {Σ} `{anerisPreG Σ unit_model} (N: namespace) ip
+  (Φ: ∀ `{anerisG Σ}, iProp Σ → val → iProp Σ)  (* Module specification *)
+  (P0: iProp Σ) (* Initial resources required by the module *)
+  (e: val → expr) (* Context program, parameterized by the module *)
+  (e_init: expr) (* Initialization code, used to allocate resources for P0 *)
+  (imimpl: val) (* Implementation of the module (instrumented) *)
+  (good_trace: list val → Prop) (* Trace property *)
+  (σ: state): (* Initial state *)
+  (* The initial trace must satisfy the property *)
+  good_trace (state_trace σ) →
+  (* The context must be safe, given a module satisfying the specification Φ *)
+  (⊢ ∀ `(anerisG Σ) P m, Φ P m -∗ {{{ P }}} e m @[ip] {{{ v, RET v; True }}}) →
+  (* The initialization code must provide P0 *)
+  (⊢ ∀ `(anerisG Σ), {{{ True }}} e_init @[ip] {{{ v, RET v; P0 }}}) →
+  (* The implementation provided for the module (iops) must satisfy the specification Φ.
+     On top of P0 it is given SL resources for the trace. *)
+  (⊢ ∀ `(anerisG Σ), Φ (P0 ∗ trace_is (state_trace σ) ∗ trace_inv N good_trace)%I imimpl) →
+  (* Then the trace remains good at every step *)
+  ∀ σ' e',
+    step ([(mkExpr ip (e_init ;; e imimpl))], σ) (e', σ') →
+    good_trace (state_trace σ').
+Proof.
+  intros Htrσ Hctx Hinit Himpl σ' e' Hsteps.
+  eapply heap_invariance. done.
+  2: eapply Hsteps.
+  iIntros (?) "HI Htr". wp_bind e_init.
+  iApply Hinit; first done.
+  iNext.
+  iIntros (v) "H0". wp_pures.
+  iApply (Hctx with "[] [H0 Htr HI]").
+  - iApply Himpl.
+  - iFrame.
+  - eauto.
+Qed.
